\documentclass{article}
\usepackage{epsfig}
\pagestyle{empty}
\begin{document}
$\displaystyle P(k) = {t \choose k}p^k(1-p)^{t-k}$
\pagebreak

$\displaystyle P(x) = \frac{x^{(n/2)-1}e^{-x/2}}{\Gamma(n/2)2^{n/2}}$
\pagebreak

$\displaystyle p(x) = \lambda e^{-\lambda x}$
\pagebreak

$\displaystyle p(x) = x^{\alpha-1}\frac{e^{-x/\beta}}{\beta^\alpha\Gamma(\alpha)}$
\pagebreak

$\displaystyle p(x) = \frac{1}{\sqrt{2\pi\sigma}} e^{-\frac{(x-\mu)^2}{2\sigma^2}} $
\pagebreak

$p(i) = \frac{e^{-\lambda}\lambda^i}{i!}$
\pagebreak

$\displaystyle p(x) = \frac{a}{b}\left(\frac{x}{b}\right)^{a-1}e^{-\left(\frac{x}{b}\right)^a}$
\pagebreak

\end{document}
